<?xml version="1.0"?>
<rdf:RDF xmlns="http://www.optimade.org/ontology/materials-databases/"
     xml:base="http://www.optimade.org/ontology/materials-databases/"
     xmlns:owl="http://www.w3.org/2002/07/owl#"
     xmlns:rdf="http://www.w3.org/1999/02/22-rdf-syntax-ns#"
     xmlns:xml="http://www.w3.org/XML/1998/namespace"
     xmlns:xsd="http://www.w3.org/2001/XMLSchema#"
     xmlns:mdbs="http://www.optimade.org/ontology/materials-databases/"
     xmlns:rdfs="http://www.w3.org/2000/01/rdf-schema#">
    <owl:Ontology rdf:about="http://www.optimade.org/ontology/materials-databases/">
        <rdfs:comment>Ontology for Materials Databases</rdfs:comment>
        <rdfs:label>Materials Databases Ontology</rdfs:label>
        <owl:versionInfo rdf:datatype="http://www.w3.org/2001/XMLSchema#string">0.1</owl:versionInfo>
    </owl:Ontology>
    


    <!-- 
    ///////////////////////////////////////////////////////////////////////////////////////
    //
    // Object Properties
    //
    ///////////////////////////////////////////////////////////////////////////////////////
     -->

    


    <!-- http://www.optimade.org/ontology/materials-databases/isDescribedByMaterialsModel -->

    <owl:ObjectProperty rdf:about="http://www.optimade.org/ontology/materials-databases/isDescribedByMaterialsModel">
        <rdfs:domain rdf:resource="http://www.optimade.org/ontology/materials-databases/Material"/>
        <rdfs:range rdf:resource="http://www.optimade.org/ontology/materials-databases/MaterialsModel"/>
        <rdfs:comment xml:lang="en">An isDescribedByMaterialsModel relationship states that a material is described by a materials model</rdfs:comment>
        <rdfs:label xml:lang="en">is described by materials model</rdfs:label>
    </owl:ObjectProperty>
    


    <!-- 
    ///////////////////////////////////////////////////////////////////////////////////////
    //
    // Classes
    //
    ///////////////////////////////////////////////////////////////////////////////////////
     -->

    


    <!-- http://www.optimade.org/ontology/materials-databases/AmorphousStructureMaterialsModel -->

    <owl:Class rdf:about="http://www.optimade.org/ontology/materials-databases/AmorphousStructureMaterialsModel">
        <rdfs:subClassOf rdf:resource="http://www.optimade.org/ontology/materials-databases/MaterialsModel"/>
        <rdfs:comment xml:lang="en">A composite materials model specify a material by a set of parameters that describe an amorphous structure.</rdfs:comment>
        <rdfs:label xml:lang="en">Amorphous structure materials model</rdfs:label>
    </owl:Class>
    


    <!-- http://www.optimade.org/ontology/materials-databases/CompositeMaterialsModel -->

    <owl:Class rdf:about="http://www.optimade.org/ontology/materials-databases/CompositeMaterialsModel">
        <rdfs:subClassOf rdf:resource="http://www.optimade.org/ontology/materials-databases/MaterialsModel"/>
        <rdfs:comment xml:lang="en">A composite materials model specify a material by a set of parameters that describe a composite.</rdfs:comment>
        <rdfs:label xml:lang="en">Composite materials model</rdfs:label>
    </owl:Class>
    


    <!-- http://www.optimade.org/ontology/materials-databases/Material -->

    <owl:Class rdf:about="http://www.optimade.org/ontology/materials-databases/Material">
        <rdfs:comment xml:lang="en">A material is a system of atoms in a state described by a statistical distribution over &apos;microstates&apos; (microscopic structure realizations).

A material is distinguished from other materials by the ensemble of microstates that, due to the statistical distribution, are effectively the relevant ones in observations of the system. Two systems with distinctively different ensembles of relevant microstates are two different materials.

For a system of atoms in an environment that changes (e.g. the temperature, pressure, etc.) the ensemble of relevant microstates may change. This can happen discontinuously, which represents a phase transition, or continuously over a path in the phase diagram.

The ensemble of relevant microstates may contain only a single microstate. This is, depending on the periodicity, the representation of a perfect bulk single crystal, slab, wire or molecule.

While the ensemble of relevant microstates defines the specific material, a material can be specified without explicitly specifying this ensemble of microstates via a materials model. Such models include the description of the material as a composite, a metallic alloy, an amorphous structure, a quasicrystal, or as the result of a synthesis process.</rdfs:comment>
        <rdfs:label xml:lang="en">Material</rdfs:label>
    </owl:Class>
    


    <!-- http://www.optimade.org/ontology/materials-databases/MaterialsModel -->

    <owl:Class rdf:about="http://www.optimade.org/ontology/materials-databases/MaterialsModel">
        <rdfs:label xml:lang="en">Materials model</rdfs:label>
    </owl:Class>
    


    <!-- http://www.optimade.org/ontology/materials-databases/MetallicAlloyMaterialsModel -->

    <owl:Class rdf:about="http://www.optimade.org/ontology/materials-databases/MetallicAlloyMaterialsModel">
        <rdfs:subClassOf rdf:resource="http://www.optimade.org/ontology/materials-databases/MaterialsModel"/>
        <rdfs:comment xml:lang="en">A metallic alloy materials model specify a material by a set of parameters that describe a metallic alloy.</rdfs:comment>
        <rdfs:label xml:lang="en">Metallic alloy materials model</rdfs:label>
    </owl:Class>
    


    <!-- http://www.optimade.org/ontology/materials-databases/QuasicrystalMaterialsModel -->

    <owl:Class rdf:about="http://www.optimade.org/ontology/materials-databases/QuasicrystalMaterialsModel">
        <rdfs:subClassOf rdf:resource="http://www.optimade.org/ontology/materials-databases/MaterialsModel"/>
        <rdfs:comment xml:lang="en">A composite materials model specify a material by a set of parameters that describe a quasicrystal. This is done as by defining cuts in a periodic crystal in higher dimensions.</rdfs:comment>
        <rdfs:label xml:lang="en">Quasicrystal materials model</rdfs:label>
    </owl:Class>
    


    <!-- http://www.optimade.org/ontology/materials-databases/SingleStructureMaterialsModel -->

    <owl:Class rdf:about="http://www.optimade.org/ontology/materials-databases/SingleStructureMaterialsModel">
        <rdfs:subClassOf rdf:resource="http://www.optimade.org/ontology/materials-databases/MaterialsModel"/>
        <rdfs:comment xml:lang="en">A single structure materials model is a materials model that specify the ensemble of relevant microstates of a material as a single structure. This represents, depending on the periodicity, a perfect bulk single crystal, slab, wire or molecule.</rdfs:comment>
        <rdfs:label xml:lang="en">Single structure materials model</rdfs:label>
    </owl:Class>
    


    <!-- http://www.optimade.org/ontology/materials-databases/Structure -->

    <owl:Class rdf:about="http://www.optimade.org/ontology/materials-databases/Structure">
        <rdfs:comment xml:lang="en">A structure is the geometrical configuration of specific atomic species. It may be partially or fully periodic or non-periodic.

A structure may encompass a restricted ensemble of geometric realizations to the degree that can be described by disordered occupation on specific sites, or as disordered correlated occupations as can be described as assemblies.

A structure may encompass a level of uncertainty in geometric realization with implicit atoms and site attachments.</rdfs:comment>
        <rdfs:label xml:lang="en">Structure</rdfs:label>
    </owl:Class>
    


    <!-- http://www.optimade.org/ontology/materials-databases/StructuresEnsembleMaterialsModel -->

    <owl:Class rdf:about="http://www.optimade.org/ontology/materials-databases/StructuresEnsembleMaterialsModel">
        <rdfs:subClassOf rdf:resource="http://www.optimade.org/ontology/materials-databases/MaterialsModel"/>
        <rdfs:comment xml:lang="en">A structures ensemble materials model is a materials model that explicitly specify a set of structures as forming the ensemble of relevant microstates of the material.</rdfs:comment>
        <rdfs:label xml:lang="en">Structures ensemble materials model</rdfs:label>
    </owl:Class>
    


    <!-- http://www.optimade.org/ontology/materials-databases/SynthesisDescriptionMaterialsModel -->

    <owl:Class rdf:about="http://www.optimade.org/ontology/materials-databases/SynthesisDescriptionMaterialsModel">
        <rdfs:subClassOf rdf:resource="http://www.optimade.org/ontology/materials-databases/MaterialsModel"/>
        <rdfs:comment xml:lang="en">A synthesis description materials model specify a material by a set of synthesis steps that, when followed, results in the synthesis of the material.</rdfs:comment>
        <rdfs:label xml:lang="en">Synthesis description materials model</rdfs:label>
    </owl:Class>
</rdf:RDF>



<!-- Generated by the OWL API (version 4.5.9.2019-02-01T07:24:44Z) https://github.com/owlcs/owlapi -->

